does not build - working...

z-match.dfy
@@ -1,12 +1,43 @@
+/* Array Predicates */
+
 predicate nonempty <T> (arr : array<T>)
 {
   arr != null && 0 < arr.Length
 }
 
 predicate same_size <S, T> (arr1 : array<S>, arr2 : array<T>)
+  requires nonempty(arr1)
+  requires nonempty(arr2)
 {
-  nonempty(arr1) && nonempty(arr2) && arr1.Length == arr2.Length
+  arr1.Length == arr2.Length
 }
+
+predicate valid_idx <T> (idx : int, arr : array<T>)
+  requires nonempty(arr)
+{
+  0 <= idx < arr.Length
+}
+
+/* NOTE: Maybe slices could be a record? Not worth it right now. */
+
+predicate valid_slice <T> (start : int, size : int, arr : array<T>)
+  requires nonempty(arr)
+{
+  forall idx :: start <= idx < start + size ==> valid_idx(idx, arr)
+}
+/*
+predicate slice_eq <T(==)> (start1 : int, arr1 : array<T>, start2 : int, arr2 : array<T>, size : int)
+  reads arr1
+  reads arr2
+  requires nonempty(arr1)
+  requires nonempty(arr2)
+  requires valid_slice(start1, size, arr1)
+  requires valid_slice(start2, size, arr2)
+{
+  forall offset :: 0 <= offset < size ==> arr1[start1] == arr2[start2]
+}
+*/
+/* Z Predicates */
 
 predicate z_zero_correct (zs : array<int>)
   reads zs
@@ -26,14 +57,14 @@ predicate z_nonzero_correct(str : array<char>, zs : array<int>)
 
 method z_algorithm_naive(str : array<char>) returns (zs : array<int>)
   requires nonempty(str)
-  
+
   ensures same_size(str, zs)
   ensures z_zero_correct(zs)
   ensures forall k :: 1 <= k < zs.Length ==> k + zs[k] <= zs.Length // TODO: Add Z's sanity check predicate
   ensures z_nonzero_correct(str, zs)
 { // TODO: Refactor invariants as predicates
   zs := new int[str.Length];
-  
+
   zs[0] := 0;
 
   var i := 1;
@@ -61,4 +92,124 @@ method z_algorithm_naive(str : array<char>) returns (zs : array<int>)
 
     i := i + 1;
   }
+}
+
+method z_algorithm(str : array<char>) returns (zs : array<int>)
+  requires nonempty(str)
+  ensures same_size(str, zs)
+  ensures z_zero_correct(zs)
+  ensures forall k :: 1 <= k < zs.Length ==> k + zs[k] <= zs.Length // TODO: Add Z's sanity check predicate
+  ensures z_nonzero_correct(str, zs)
+{
+  zs := new int[str.Length];
+  zs[0] := 0;
+  var maxZ := 0;
+  var j := 0;
+  var i := 1;
+  
+  while (i< zs.Length)
+    invariant 1 <= i <= zs.Length
+    invariant z_zero_correct(zs)
+    invariant j < i
+    invariant forall k :: 1 <= k < i ==> k + zs[k] <= zs.Length
+    invariant j+zs[j] == maxZ
+    invariant maxZ <= zs.Length
+    invariant forall k :: 1 <= k < i ==> forall l :: 0 <= l < zs[k] ==> str[l] == str[k + l]
+  {
+    if (maxZ < i){
+      var l := 0;
+      zs[i] := 0;
+      
+      while (i+l<str.Length) && (str[i+l]==str[l])
+        invariant 1 <= i+l <= str.Length
+        invariant forall k :: 1 <= k < i ==> k + zs[k] <= zs.Length
+        invariant i+zs[i] <= zs.Length
+        invariant zs[i] == l
+        invariant z_zero_correct(zs)
+        invariant maxZ <= zs.Length
+        invariant forall k :: 1 <= k < i ==> forall l :: 0 <= l < zs[k] ==> str[l] == str[k + l]
+        invariant forall m :: 0 <= m < zs[i] ==> str[m] == str[i+m]
+      {
+        zs[i] := zs[i]+1;
+        l := l+1;  
+      }
+      maxZ := i+zs[i];
+      j:= i;
+    }
+    else{
+      assert (i <= j + zs[j]);
+      var k := i-j;
+      if (zs[k]+i < maxZ){ // case 1
+        zs[i] := zs[k];
+      }
+      else if (zs[k]+i>maxZ){ // case 2
+        zs[i] := maxZ-i;
+      }
+      else { // case 3: zs[k]+i == maxZ 
+        zs[i] := maxZ-i;
+        var l := zs[i];
+        while (i+l<str.Length) && (str[i+l]==str[l])
+            invariant 1 <= i <= zs.Length
+            invariant z_zero_correct(zs)
+            invariant forall k :: 1 <= k < i ==> k + zs[k] <= zs.Length
+            invariant maxZ <= zs.Length
+            invariant i+zs[i] <= zs.Length
+            invariant zs[i] == l
+            invariant forall k :: 1 <= k < i ==> forall l :: 0 <= l < zs[k] ==> str[l] == str[k + l]
+            invariant forall m :: 0 <= m < zs[i] ==> str[m] == str[i+m]
+        {
+          zs[i] := zs[i]+1;
+          l := l+1;
+        }
+        maxZ := i+zs[i];
+        j:=i;
+      }
+    }
+    i := i+1;
+  }
+}
+
+method print_arr <T> (arr : array<T>)
+  requires nonempty(arr)
+{
+  var i := 0;
+
+  print "[";
+
+  while (i < arr.Length - 1)
+    invariant 0 <= i <= arr.Length - 1
+  {
+    print arr[i];
+    print " ";
+
+    i := i + 1;
+  }
+
+  print arr[i];
+  print "]\n";
+}
+
+method array_of_string (str : string) returns (ret : array<char>)
+  requires 0 < |str|
+
+  ensures nonempty(ret)
+{
+  ret := new char[|str|];
+
+  var i := 0;
+
+  while (i < |str|)
+  {
+    ret[i] := str[i];
+
+    i := i + 1;
+  }
+}
+
+method Main() {
+  var str := "heheh";
+  var str_as_arr := array_of_string(str);
+  print_arr(str_as_arr);
+  var res := z_algorithm(str_as_arr);
+  print_arr(res);
 }
